PREFIX cs: <https://prez.dev/ManifestResourceRoles>
PREFIX mrr: <https://prez.dev/ManifestResourceRoles/>
PREFIX owl: <http://www.w3.org/2002/07/owl#>
PREFIX rdfs: <http://www.w3.org/2000/01/rdf-schema#>
PREFIX schema: <https://schema.org/>
PREFIX skos: <http://www.w3.org/2004/02/skos/core#>
PREFIX xsd: <http://www.w3.org/2001/XMLSchema#>

mrr:contentModel
    a skos:Concept ;
    skos:definition "The default model for the content. Must be a set of SAHCL Shapes" ;
    skos:inScheme cs: ;
    skos:prefLabel "Content Model" ;
.

mrr:CompleteContainerAndContentLabels
    a skos:Concept ;
    skos:definition "All the labels - possibly indluding names, descriptions & seeAlso links - for the Container and Content objects" ;
    skos:inScheme cs: ;
    skos:prefLabel "Complete Content and Container Labels" ;
.

mrr:ContainerAndContentModel
    a skos:Concept ;
    skos:definition "The default model for the container and the content. Must be a set of SAHCL Shapes" ;
    skos:inScheme cs: ;
    skos:prefLabel "Container & Content Model" ;
.

mrr:ContainerData
    a skos:Concept ;
    skos:definition "Data for the container, usually a Catalogue, including the identity of it and each item fo content" ;
    skos:inScheme cs: ;
    skos:prefLabel "Container Data" ;
.

mrr:ContainerModel
    a skos:Concept ;
    skos:definition "The default model for the container. Must be a set of SAHCL Shapes" ;
    skos:inScheme cs: ;
    skos:prefLabel "Container Model" ;
.

mrr:ContentData
    a skos:Concept ;
    skos:definition "Data for the content of the container" ;
    skos:inScheme cs: ;
    skos:prefLabel "Content Data" ;
.

mrr:IncompleteContainerAndContentLabels
    a skos:Concept ;
    skos:definition "Some of the labels - possibly indluding names, descriptions & seeAlso links - for the Container and Content objects" ;
    skos:inScheme cs: ;
    skos:prefLabel "Incomplete Content and Container Labels" ;
.

<https://kurrawong.ai>
    a schema:Organization ;
    schema:name "KurrawongAI" ;
    schema:url "https://kurrawong.ai"^^xsd:anyURI ;
.

mrr:1.0.0
    rdfs:label "1.0.0" ;
.

cs:
    a skos:ConceptScheme ;
    owl:versionIRI mrr:1.0.0 ;
    owl:versionInfo "1.0.0: First public version" ;
    skos:definition "This vocabulary is a test vocabulary showing the use of images within Concept definitions"@en ;
    skos:hasTopConcept
        mrr:completeContainerAndContentLabels ,
        mrr:containerAndContentModel ,
        mrr:containerData ,
        mrr:containerModel ,
        mrr:contentData ,
        mrr:incompleteContainerAndContentLabels ;
    skos:historyNote "Create in 2024 for Prez data loading" ;
    skos:prefLabel "Manifest Resource Roles Vocabulary" ;
    schema:creator <https://kurrawong.ai> ;
    schema:dateCreated "2024-11-29"^^xsd:date ;
    schema:dateModified "2024-11-29"^^xsd:date ;
    schema:publisher <https://kurrawong.ai> ;
.